chore: add `ReaderT.mk` and `StateT.mk`
These complement the existing `ExceptT.mk` and `OptionT.mk`, and provide a symbol to key `simp` lemmas on, to prevent getting stuck on `(StateT.run fun s => f s) s`.

A future PR could insert these new `mk`s into the implementation of many definitions, such that unfolding the definitions leaves appropriate casts behind; but this is invasive, and by itself having `mk` provides value.

src/Init/Prelude.lean
@@ -4035,6 +4035,12 @@ ordinary actions in `m`.
 def ReaderT (ρ : Type u) (m : Type u → Type v) (α : Type u) : Type (max u v) :=
   ρ → m α
 
+/--
+Interpret `ρ → m α` as an element of `ReaderT ρ m α`.
+-/
+@[always_inline, inline]
+def ReaderT.mk {ρ : Type u} {m : Type u → Type v} {α : Type u} (x : ρ → m α) : ReaderT ρ m α := x
+
 instance (ρ : Type u) (m : Type u → Type v) (α : Type u) [Inhabited (m α)] : Inhabited (ReaderT ρ m α) where
   default := fun _ => default
 
